RISC-V: expand with User mode support

case_study/RiscvPmp/Machine.v
@@ -86,6 +86,10 @@ Module RiscvPmpTermKit <: TermKit.
   Local Notation "'c'"            := "c" : string_scope.
   Local Notation "'cause'"        := "cause" : string_scope.
   Local Notation "'m'"            := "m" : string_scope.
+  Local Notation "'priv'"         := "priv" : string_scope.
+  Local Notation "'cur_priv'"     := "cur_priv" : string_scope.
+  Local Notation "'del_priv'"     := "del_priv" : string_scope.
+  Local Notation "'p'"            := "p" : string_scope.
 
   (** Functions **)
   Inductive Fun : PCtx -> Ty -> Set :=
@@ -98,17 +102,17 @@ Module RiscvPmpTermKit <: TermKit.
   | mem_read              : Fun [typ ∶ ty_access_type, paddr ∶ ty_int] ty_memory_op_result
   | checked_mem_read      : Fun [t ∶ ty_access_type, paddr ∶ ty_int] ty_memory_op_result
   | checked_mem_write     : Fun [paddr ∶ ty_int, data ∶ ty_word] ty_memory_op_result
-  | pmp_mem_read          : Fun [t∶ ty_access_type, paddr ∶ ty_int] ty_memory_op_result
-  | pmp_mem_write         : Fun [paddr ∶ ty_int, data ∶ ty_word, typ ∶ ty_access_type] ty_memory_op_result
+  | pmp_mem_read          : Fun [t∶ ty_access_type, p ∶ ty_privilege, paddr ∶ ty_int] ty_memory_op_result
+  | pmp_mem_write         : Fun [paddr ∶ ty_int, data ∶ ty_word, typ ∶ ty_access_type, priv ∶ ty_privilege] ty_memory_op_result
   | pmpLocked             : Fun [cfg ∶ ty_pmpcfg_ent] ty_bool
-  | pmpCheck              : Fun [addr ∶ ty_int, acc ∶ ty_access_type] (ty_option ty_exception_type)
-  | pmpCheckPerms         : Fun [ent ∶ ty_pmpcfg_ent, acc ∶ ty_access_type] ty_bool
+  | pmpCheck              : Fun [addr ∶ ty_int, acc ∶ ty_access_type, priv ∶ ty_privilege] (ty_option ty_exception_type)
+  | pmpCheckPerms         : Fun [ent ∶ ty_pmpcfg_ent, acc ∶ ty_access_type, priv ∶ ty_privilege] ty_bool
   | pmpCheckRWX           : Fun [ent ∶ ty_pmpcfg_ent, acc ∶ ty_access_type] ty_bool
-  | pmpMatchEntry         : Fun [addr ∶ ty_int, acc ∶ ty_access_type, ent ∶ ty_pmpcfg_ent, pmpaddr ∶ ty_int, prev_pmpaddr ∶ ty_int] ty_pmpmatch
+  | pmpMatchEntry         : Fun [addr ∶ ty_int, acc ∶ ty_access_type, priv ∶ ty_privilege, ent ∶ ty_pmpcfg_ent, pmpaddr ∶ ty_int, prev_pmpaddr ∶ ty_int] ty_pmpmatch
   | pmpAddrRange          : Fun [cfg ∶ ty_pmpcfg_ent, pmpaddr ∶ ty_int, prev_pmpaddr ∶ ty_int] ty_pmp_addr_range
   | pmpMatchAddr          : Fun [addr ∶ ty_int, rng ∶ ty_pmp_addr_range] ty_pmpaddrmatch
   | process_load          : Fun [rd ∶ ty_regidx, vaddr ∶ ty_int, value ∶ ty_memory_op_result] ty_retired
-  | write_mem_value       : Fun [paddr ∶ ty_int, value ∶ ty_word] ty_memory_op_result
+  | mem_write_value       : Fun [paddr ∶ ty_int, value ∶ ty_word] ty_memory_op_result
   | main                  : Fun ctx_nil ty_unit
   | init_model            : Fun ctx_nil ty_unit
   | loop                  : Fun ctx_nil ty_unit
@@ -118,10 +122,12 @@ Module RiscvPmpTermKit <: TermKit.
   | init_pmp              : Fun ctx_nil ty_unit
   | exceptionType_to_bits : Fun [e ∶ ty_exception_type] ty_exc_code
   | handle_mem_exception  : Fun [addr ∶ ty_int, e ∶ ty_exception_type] ty_unit
-  | exception_handler     : Fun [ctl ∶ ty_ctl_result, "pc" ∶ ty_int] ty_int
-  | trap_handler          : Fun [c ∶ ty_exc_code, "pc" ∶ ty_int] ty_int
-  | prepare_trap_vector   : Fun [cause ∶ ty_mcause] ty_int
+  | exception_handler     : Fun [cur_priv ∶ ty_privilege, ctl ∶ ty_ctl_result, "pc" ∶ ty_int] ty_int
+  | exception_delegatee   : Fun [p ∶ ty_privilege] ty_privilege
+  | trap_handler          : Fun [del_priv ∶ ty_privilege, c ∶ ty_exc_code, "pc" ∶ ty_int] ty_int
+  | prepare_trap_vector   : Fun [p ∶ ty_privilege, cause ∶ ty_mcause] ty_int
   | tvec_addr             : Fun [m ∶ ty_int, c ∶ ty_mcause] (ty_option ty_int)
+  | handle_illegal        : Fun ctx_nil ty_unit
   | execute_RTYPE         : Fun [rs2 ∶ ty_regidx, rs1 ∶ ty_regidx, rd ∶ ty_regidx, op ∶ ty_rop] ty_retired
   | execute_ITYPE         : Fun [imm ∶ ty_int, rs1 ∶ ty_regidx, rd ∶ ty_regidx, op ∶ ty_iop] ty_retired
   | execute_UTYPE         : Fun [imm ∶ ty_int, rd ∶ ty_regidx, op ∶ ty_uop] ty_retired
@@ -130,6 +136,8 @@ Module RiscvPmpTermKit <: TermKit.
   | execute_RISCV_JALR    : Fun [imm ∶ ty_int, rs1 ∶ ty_regidx, rd ∶ ty_regidx] ty_retired
   | execute_LOAD          : Fun [imm ∶ ty_int, rs1 ∶ ty_regidx, rd ∶ ty_regidx] ty_retired
   | execute_STORE         : Fun [imm ∶ ty_int, rs2 ∶ ty_regidx, rs1 ∶ ty_regidx] ty_retired
+  | execute_ECALL         : Fun ctx_nil ty_retired
+  | execute_MRET          : Fun ctx_nil ty_retired
   .
 
   Inductive FunX : PCtx -> Ty -> Set :=
@@ -145,16 +153,18 @@ Module RiscvPmpTermKit <: TermKit.
   Definition 𝑳  : PCtx -> Set := Lem.
 
   Inductive Reg : Ty -> Set :=
-  | pc       : Reg ty_word
-  | nextpc   : Reg ty_word
-  | mtvec    : Reg ty_word
-  | mcause   : Reg ty_exc_code
-  | mepc     : Reg ty_word
-  | x0       : Reg ty_word
-  | x1       : Reg ty_word
-  | x2       : Reg ty_word
-  | pmp0cfg  : Reg ty_pmpcfg_ent
-  | pmpaddr0 : Reg ty_int
+  | pc            : Reg ty_word
+  | nextpc        : Reg ty_word
+  | mstatus       : Reg ty_mstatus
+  | mtvec         : Reg ty_word
+  | mcause        : Reg ty_exc_code
+  | mepc          : Reg ty_word
+  | cur_privilege : Reg ty_privilege
+  | x0            : Reg ty_word
+  | x1            : Reg ty_word
+  | x2            : Reg ty_word
+  | pmp0cfg       : Reg ty_pmpcfg_ent
+  | pmpaddr0      : Reg ty_int
   .
 
   Section TransparentObligations.
@@ -177,7 +187,7 @@ Module RiscvPmpTermKit <: TermKit.
     intros xy; eapply 𝑹𝑬𝑮_eq_dec.
   Defined.
 
-  Program Instance 𝑹𝑬𝑮_finite : Finite (sigT Reg) := {| enum := [ existT _ pc; existT _ nextpc; existT _ mtvec; existT _ mcause; existT _ mepc; existT _ x0; existT _ x1; existT _ x2; existT _ pmp0cfg; existT _ pmpaddr0 ]%list |}.
+  Program Instance 𝑹𝑬𝑮_finite : Finite (sigT Reg) := {| enum := [ existT _ pc; existT _ nextpc; existT _ mstatus; existT _ mtvec; existT _ mcause; existT _ mepc; existT _ cur_privilege; existT _ x0; existT _ x1; existT _ x2; existT _ pmp0cfg; existT _ pmpaddr0 ]%list |}.
   Next Obligation.
     now eapply (nodup_fixed (H := 𝑹𝑬𝑮_eq_dec)).
   Defined.
@@ -186,7 +196,6 @@ Module RiscvPmpTermKit <: TermKit.
     refine (@bool_decide_unpack _ (elem_of_list_dec _ _) _).
     destruct x; now destruct r.
   Qed.
-
 
 End RiscvPmpTermKit.
 
@@ -247,6 +256,12 @@ Module RiscvPmpProgramKit <: (ProgramKit RiscvPmpTermKit).
   Local Notation "'tvec'"         := "tvec" : string_scope.
   Local Notation "'m'"            := "m" : string_scope.
   Local Notation "'epc'"          := "epc" : string_scope.
+  Local Notation "'priv'"         := "priv" : string_scope.
+  Local Notation "'cur_priv'"     := "cur_priv" : string_scope.
+  Local Notation "'del_priv'"     := "del_priv" : string_scope.
+  Local Notation "'prev_priv'"    := "prev_priv" : string_scope.
+  Local Notation "'p'"            := "p" : string_scope.
+  Local Notation "'MPP'"          := "MPP" : string_scope.
 
   Local Notation "'rs'"           := (@exp_var _ "rs" _ _) : exp_scope.
   Local Notation "'rs1'"          := (@exp_var _ "rs1" _ _) : exp_scope.
@@ -299,6 +314,12 @@ Module RiscvPmpProgramKit <: (ProgramKit RiscvPmpTermKit).
   Local Notation "'tvec'"         := (@exp_var _ "tvec" _ _) : exp_scope.
   Local Notation "'m'"            := (@exp_var _ "m" _ _) : exp_scope.
   Local Notation "'epc'"          := (@exp_var _ "epc" _ _) : exp_scope.
+  Local Notation "'priv'"         := (@exp_var _ "priv" _ _) : exp_scope.
+  Local Notation "'cur_priv'"     := (@exp_var _ "cur_priv" _ _) : exp_scope.
+  Local Notation "'del_priv'"     := (@exp_var _ "del_priv" _ _) : exp_scope.
+  Local Notation "'prev_priv'"    := (@exp_var _ "prev_priv" _ _) : exp_scope.
+  Local Notation "'p'"            := (@exp_var _ "p" _ _) : exp_scope.
+  Local Notation "'MPP'"          := (@exp_var _ "MPP" _ _) : exp_scope.
 
   Local Notation "'Read'" := (exp_union access_type KRead (exp_lit ty_unit tt)) : exp_scope.
   Local Notation "'Write'" := (exp_union access_type KWrite (exp_lit ty_unit tt)) : exp_scope.
@@ -308,6 +329,9 @@ Module RiscvPmpProgramKit <: (ProgramKit RiscvPmpTermKit).
   Local Notation "'E_Fetch_Access_Fault'" := (exp_union exception_type KE_Fetch_Access_Fault (exp_lit ty_unit tt)) : exp_scope.
   Local Notation "'E_Load_Access_Fault'" := (exp_union exception_type KE_Load_Access_Fault (exp_lit ty_unit tt)) : exp_scope.
   Local Notation "'E_SAMO_Access_Fault'" := (exp_union exception_type KE_SAMO_Access_Fault (exp_lit ty_unit tt)) : exp_scope.
+  Local Notation "'E_U_EnvCall'" := (exp_union exception_type KE_U_EnvCall (exp_lit ty_unit tt)) : exp_scope.
+  Local Notation "'E_M_EnvCall'" := (exp_union exception_type KE_M_EnvCall (exp_lit ty_unit tt)) : exp_scope.
+  Local Notation "'E_Illegal_Instr'" := (exp_union exception_type KE_Illegal_Instr (exp_lit ty_unit tt)) : exp_scope.
 
   Local Notation "'None'" := (exp_inr (exp_lit ty_unit tt)) : exp_scope.
   Local Notation "'Some' va" := (exp_inl va) (at level 10, va at next level) : exp_scope.
@@ -319,6 +343,7 @@ Module RiscvPmpProgramKit <: (ProgramKit RiscvPmpTermKit).
   Local Notation "'F_Error' meme memv" := (exp_union fetch_result KF_Error (exp_binop binop_pair meme memv)) (at level 10, meme at next level, memv at next level) : exp_scope.
 
   Local Notation "'CTL_TRAP' exc" := (exp_union ctl_result KCTL_TRAP exc) (at level 10, exc at next level) : exp_scope.
+  Local Notation "'CTL_MRET'" := (exp_union ctl_result KCTL_MRET (exp_lit ty_unit tt)) : exp_scope.
 
   (** Functions **)
   Definition fun_rX : Stm [rs ∶ ty_regidx] ty_word :=
@@ -351,7 +376,8 @@ Module RiscvPmpProgramKit <: (ProgramKit RiscvPmpTermKit).
     else v.
 
   Definition fun_mem_read : Stm [typ ∶ ty_access_type, paddr ∶ ty_int] ty_memory_op_result :=
-    call pmp_mem_read typ paddr.
+    let: tmp := stm_read_register cur_privilege in
+    call pmp_mem_read typ tmp paddr.
 
   Definition fun_checked_mem_read : Stm [t ∶ ty_access_type, paddr ∶ ty_int] ty_memory_op_result :=
     let: tmp := foreign read_ram paddr in
@@ -361,22 +387,22 @@ Module RiscvPmpProgramKit <: (ProgramKit RiscvPmpTermKit).
     let: tmp := foreign write_ram paddr data in
     MemValue tmp.
 
-  Definition fun_pmp_mem_read : Stm [t∶ ty_access_type, paddr ∶ ty_int] ty_memory_op_result :=
-    let: tmp := call pmpCheck paddr t in
+  Definition fun_pmp_mem_read : Stm [t∶ ty_access_type, p ∶ ty_privilege, paddr ∶ ty_int] ty_memory_op_result :=
+    let: tmp := call pmpCheck paddr t p in
     match: tmp with
     | inl e => MemException e
     | inr v => call checked_mem_read t paddr
     end.
 
-  Definition fun_pmp_mem_write : Stm [paddr ∶ ty_int, data ∶ ty_word, typ ∶ ty_access_type] ty_memory_op_result :=
-    let: tmp := call pmpCheck paddr typ in
+  Definition fun_pmp_mem_write : Stm [paddr ∶ ty_int, data ∶ ty_word, typ ∶ ty_access_type, priv ∶ ty_privilege] ty_memory_op_result :=
+    let: tmp := call pmpCheck paddr typ priv in
     match: tmp with
     | inl e => MemException e
     | inr v => call checked_mem_write paddr data
     end.
 
   Definition fun_pmpLocked : Stm [cfg ∶ ty_pmpcfg_ent] ty_bool :=
-    (stm_match_record pmpcfg_ent cfg
+    (stm_match_record rpmpcfg_ent cfg
       (recordpat_snoc (recordpat_snoc (recordpat_snoc (recordpat_snoc (recordpat_snoc recordpat_nil
        "L" L)
        "A" A)
@@ -385,14 +411,17 @@ Module RiscvPmpProgramKit <: (ProgramKit RiscvPmpTermKit).
        "R" R)
       L).
 
-  Definition fun_pmpCheck : Stm [addr ∶ ty_int, acc ∶ ty_access_type] (ty_option ty_exception_type) :=
+  Definition fun_pmpCheck : Stm [addr ∶ ty_int, acc ∶ ty_access_type, priv ∶ ty_privilege] (ty_option ty_exception_type) :=
     let: tmp1 := stm_read_register pmp0cfg in
     let: tmp2 := stm_read_register pmpaddr0 in
-    let: tmp3 := call pmpMatchEntry addr acc tmp1 tmp2 (exp_lit ty_int 0%Z) in
+    let: tmp3 := call pmpMatchEntry addr acc priv tmp1 tmp2 (exp_lit ty_int 0%Z) in
     let: check%string := match: tmp3 in pmpmatch with
                   | PMP_Success  => stm_lit ty_bool true
                   | PMP_Fail     => stm_lit ty_bool false
-                  | PMP_Continue => stm_lit ty_bool true
+                  | PMP_Continue => match: priv in privilege with
+                                    | Machine => stm_lit ty_bool true
+                                    | User    => stm_lit ty_bool false
+                                    end
                   end in
            if: check
            then None
@@ -410,15 +439,19 @@ Module RiscvPmpProgramKit <: (ProgramKit RiscvPmpTermKit).
                                                      (Some E_Fetch_Access_Fault)
                                     end).
 
-  Definition fun_pmpCheckPerms : Stm [ent ∶ ty_pmpcfg_ent, acc ∶ ty_access_type] ty_bool :=
-    let: tmp := call pmpLocked ent in
-    if: tmp
-    then let: tmp := call pmpCheckRWX ent acc in
-         tmp
-    else stm_lit ty_bool true.
+  Definition fun_pmpCheckPerms : Stm [ent ∶ ty_pmpcfg_ent, acc ∶ ty_access_type, priv ∶ ty_privilege] ty_bool :=
+    match: priv in privilege with
+    | Machine =>
+      let: tmp := call pmpLocked ent in
+      if: tmp
+      then call pmpCheckRWX ent acc
+      else stm_lit ty_bool true
+    | User =>
+      call pmpCheckRWX ent acc
+    end.
 
   Definition fun_pmpCheckRWX : Stm [ent ∶ ty_pmpcfg_ent, acc ∶ ty_access_type] ty_bool :=
-    (stm_match_record pmpcfg_ent ent
+    (stm_match_record rpmpcfg_ent ent
       (recordpat_snoc (recordpat_snoc (recordpat_snoc (recordpat_snoc (recordpat_snoc recordpat_nil
        "L" L)
        "A" A)
@@ -438,21 +471,21 @@ Module RiscvPmpProgramKit <: (ProgramKit RiscvPmpTermKit).
                                                     X
                               end))).
 
-  Definition fun_pmpMatchEntry : Stm [addr ∶ ty_int, acc ∶ ty_access_type, ent ∶ ty_pmpcfg_ent, pmpaddr ∶ ty_int, prev_pmpaddr ∶ ty_int] ty_pmpmatch :=
+  Definition fun_pmpMatchEntry : Stm [addr ∶ ty_int, acc ∶ ty_access_type, priv ∶ ty_privilege, ent ∶ ty_pmpcfg_ent, pmpaddr ∶ ty_int, prev_pmpaddr ∶ ty_int] ty_pmpmatch :=
     let: rng := call pmpAddrRange ent pmpaddr prev_pmpaddr in
     let: tmp := call pmpMatchAddr addr rng in
     match: tmp in pmpaddrmatch with
     | PMP_NoMatch      => exp_lit ty_pmpmatch PMP_Continue
     | PMP_PartialMatch => exp_lit ty_pmpmatch PMP_Fail
     | PMP_Match        =>
-      let: tmp := call pmpCheckPerms ent acc in
+      let: tmp := call pmpCheckPerms ent acc priv in
       if: tmp
       then exp_lit ty_pmpmatch PMP_Success
       else exp_lit ty_pmpmatch PMP_Fail
     end.
 
   Definition fun_pmpAddrRange : Stm [cfg ∶ ty_pmpcfg_ent, pmpaddr ∶ ty_int, prev_pmpaddr ∶ ty_int] ty_pmp_addr_range :=
-    (stm_match_record pmpcfg_ent cfg
+    (stm_match_record rpmpcfg_ent cfg
       (recordpat_snoc (recordpat_snoc (recordpat_snoc (recordpat_snoc (recordpat_snoc recordpat_nil
        "L" L)
        "A" A)
@@ -493,8 +526,9 @@ Module RiscvPmpProgramKit <: (ProgramKit RiscvPmpTermKit).
                                                      stm_lit ty_retired RETIRE_FAIL)
                            end).
 
-  Definition fun_write_mem_value : Stm [paddr ∶ ty_int, value ∶ ty_word] ty_memory_op_result :=
-    call pmp_mem_write paddr value Write.
+  Definition fun_mem_write_value : Stm [paddr ∶ ty_int, value ∶ ty_word] ty_memory_op_result :=
+    let: tmp := stm_read_register cur_privilege in
+    call pmp_mem_write paddr value Write tmp.
 
   Definition fun_main : Stm ctx_nil ty_unit :=
     call init_model ;;
@@ -541,14 +575,14 @@ Module RiscvPmpProgramKit <: (ProgramKit RiscvPmpTermKit).
 
   Definition fun_init_pmp : Stm ctx_nil ty_unit :=
     let: tmp := stm_read_register pmp0cfg in
-    (stm_match_record pmpcfg_ent tmp
+    (stm_match_record rpmpcfg_ent tmp
       (recordpat_snoc (recordpat_snoc (recordpat_snoc (recordpat_snoc (recordpat_snoc recordpat_nil
        "L" L%string)
        "A" A%string)
        "X" X%string)
        "W" W%string)
        "R" R%string)
-      (stm_write_register pmp0cfg (exp_record pmpcfg_ent
+      (stm_write_register pmp0cfg (exp_record rpmpcfg_ent
                                              [ L,
                                                exp_lit ty_pmpaddrmatchtype OFF,
                                                X,
@@ -562,29 +596,57 @@ Module RiscvPmpProgramKit <: (ProgramKit RiscvPmpTermKit).
                            match K with
                            | KE_Fetch_Access_Fault => MkAlt pat_unit
                                                             (stm_lit ty_exc_code 1%Z)
+                           | KE_Illegal_Instr      => MkAlt pat_unit
+                                                            (stm_lit ty_exc_code 2%Z)
                            | KE_Load_Access_Fault  => MkAlt pat_unit
                                                             (stm_lit ty_exc_code 5%Z)
                            | KE_SAMO_Access_Fault  => MkAlt pat_unit
                                                             (stm_lit ty_exc_code 7%Z)
+                           | KE_U_EnvCall          => MkAlt pat_unit
+                                                            (stm_lit ty_exc_code 8%Z)
+                           | KE_M_EnvCall          => MkAlt pat_unit
+                                                            (stm_lit ty_exc_code 11%Z)
                            end).
 
   Definition fun_handle_mem_exception : Stm [addr ∶ ty_int, e ∶ ty_exception_type] ty_unit :=
     let: tmp1 := stm_read_register pc in
-    let: tmp2 := call exception_handler (CTL_TRAP e) tmp1 in
-    call set_next_pc tmp2.
+    let: tmp2 := stm_read_register cur_privilege in
+    let: tmp3 := call exception_handler tmp2 (CTL_TRAP e) tmp1 in
+    call set_next_pc tmp3.
 
-  Definition fun_exception_handler : Stm [ctl ∶ ty_ctl_result, "pc" ∶ ty_int] ty_int :=
+  Definition fun_exception_handler : Stm [cur_priv ∶ ty_privilege, ctl ∶ ty_ctl_result, "pc" ∶ ty_int] ty_int :=
     stm_match_union_alt ctl_result ctl
                         (fun K =>
                            match K with
                            | KCTL_TRAP => MkAlt (pat_var e%string)
-                                                (let: tmp := call exceptionType_to_bits e in
-                                                  call trap_handler tmp (exp_var "pc"))
+                                                (let: del_priv := call exception_delegatee cur_priv in
+                                                 let: tmp := call exceptionType_to_bits e in
+                                                 call trap_handler del_priv tmp (exp_var "pc"))
+                           | KCTL_MRET => MkAlt pat_unit
+                                                (* NOTE: normally the return address is computed with:
+                                                         prepare_xret_target(Machine) & pc_alignment_mask()
+                                                         
+                                                         we drop the alignment mask and inline prepare_xret_target,
+                                                         which just calls get_xret_target, which returns (for M-mode)
+                                                         the value of mepc *)
+                                                (let: prev_priv := stm_read_register cur_privilege in
+                                                 let: tmp1 := stm_read_register mstatus in
+                                                 (stm_match_record rmstatus tmp1
+                                                                   (recordpat_snoc recordpat_nil "MPP" MPP%string)
+                                                                   (stm_write_register cur_privilege MPP ;;
+                                                                    stm_write_register mstatus (exp_record rmstatus [ exp_lit ty_privilege User ]) ;;
+                                                                    stm_read_register mepc)))
                            end).
 
-  Definition fun_trap_handler : Stm [c ∶ ty_exc_code, "pc" ∶ ty_int] ty_int :=
+  Definition fun_exception_delegatee : Stm [p ∶ ty_privilege] ty_privilege :=
+    stm_lit ty_privilege Machine.
+
+  Definition fun_trap_handler : Stm [del_priv ∶ ty_privilege, c ∶ ty_exc_code, "pc" ∶ ty_int] ty_int :=
     stm_write_register mcause c ;;
+    let: tmp := stm_read_register cur_privilege in
+    stm_write_register mstatus (exp_record rmstatus [ tmp ]) ;;
     stm_write_register mepc (exp_var "pc") ;;
+    stm_write_register cur_privilege del_priv ;;
     (* NOTE: the following let can be dropped by just reusing c (the value we are
              writing into mcause, but this (manual) translation is more faithful to
              what I expect an automatic translation would produce, i.e. do an 
@@ -600,14 +662,17 @@ Module RiscvPmpProgramKit <: (ProgramKit RiscvPmpTermKit).
              by mtvec will need to read the mcause register to dispatch to the
              corresponding trap handler for the cause). *)
     let: tmp := stm_read_register mcause in
-    call prepare_trap_vector tmp.
+    call prepare_trap_vector del_priv tmp.
 
-  Definition fun_prepare_trap_vector : Stm [cause ∶ ty_mcause] ty_int :=
+  Definition fun_prepare_trap_vector : Stm [p ∶ ty_privilege, cause ∶ ty_mcause] ty_int :=
     let: tvec := stm_read_register mtvec in
     let: tmp := call tvec_addr tvec cause in
     (* NOTE: tvec_addr will only ever return Some(epc), because we don't support
              the 2 mode bits and only have direct mode. The None case only arises
-             for the Reserved mode of trap vectors. *)
+             for the Reserved mode of trap vectors.
+
+             The given privilege level (p) is ignored, this only makes sense when
+             supervisor mode is supported. *)
     match: tmp with
     | inl epc => epc
     | inr e   => fail "Invalid tvec mode"
@@ -615,6 +680,13 @@ Module RiscvPmpProgramKit <: (ProgramKit RiscvPmpTermKit).
 
   Definition fun_tvec_addr : Stm [m ∶ ty_int, c ∶ ty_mcause] (ty_option ty_int) :=
     Some m.
+
+  Definition fun_handle_illegal : Stm ctx_nil ty_unit :=
+    let: t := E_Illegal_Instr in
+    let: tmp1 := stm_read_register cur_privilege in
+    let: tmp2 := stm_read_register pc in
+    let: tmp3 := call exception_handler tmp1 (CTL_TRAP t) tmp2 in
+    call set_next_pc tmp3.
 
   Definition fun_execute_RTYPE : Stm [rs2 ∶ ty_regidx, rs1 ∶ ty_regidx, rd ∶ ty_regidx, op ∶ ty_rop] ty_retired :=
     let: rs1_val := call rX rs1 in
@@ -704,7 +776,7 @@ Module RiscvPmpProgramKit <: (ProgramKit RiscvPmpTermKit).
     let: tmp := call rX rs1 in
     let: paddr := tmp + offset in
     let: rs2_val := call rX rs2 in
-    let: res := call write_mem_value paddr rs2_val in
+    let: res := call mem_write_value paddr rs2_val in
     stm_match_union_alt memory_op_result res
                         (fun K =>
                            match K with
@@ -716,6 +788,30 @@ Module RiscvPmpProgramKit <: (ProgramKit RiscvPmpTermKit).
                                                     (call handle_mem_exception paddr e ;;
                                                      stm_lit ty_retired RETIRE_FAIL)
                            end).
+
+  Definition fun_execute_ECALL : Stm ctx_nil ty_retired :=
+    let: tmp1 := stm_read_register cur_privilege in
+    let: t := match: tmp1 in privilege with
+              | Machine => E_M_EnvCall
+              | User    => E_U_EnvCall
+              end in
+    let: tmp2 := stm_read_register pc in
+    let: tmp3 := call exception_handler tmp1 (CTL_TRAP t) tmp2 in
+    call set_next_pc tmp3 ;;
+    stm_lit ty_retired RETIRE_FAIL.
+
+  Definition fun_execute_MRET : Stm ctx_nil ty_retired :=
+    let: tmp1 := stm_read_register cur_privilege in
+    match: tmp1 in privilege with
+    | Machine =>
+      let: tmp2 := stm_read_register pc in
+      let: tmp3 := call exception_handler tmp1 CTL_MRET tmp2 in
+      call set_next_pc tmp3 ;;
+      stm_lit ty_retired RETIRE_SUCCESS
+    | User    =>
+      call handle_illegal ;;
+      stm_lit ty_retired RETIRE_FAIL
+    end.
 
   End Functions.
 
@@ -772,7 +868,7 @@ Module RiscvPmpProgramKit <: (ProgramKit RiscvPmpTermKit).
     | set_next_pc           => fun_set_next_pc
     | abs                   => fun_abs
     | mem_read              => fun_mem_read
-    | write_mem_value       => fun_write_mem_value
+    | mem_write_value       => fun_mem_write_value
     | checked_mem_read      => fun_checked_mem_read
     | checked_mem_write     => fun_checked_mem_write
     | pmp_mem_read          => fun_pmp_mem_read
@@ -795,9 +891,11 @@ Module RiscvPmpProgramKit <: (ProgramKit RiscvPmpTermKit).
     | fetch                 => fun_fetch
     | handle_mem_exception  => fun_handle_mem_exception
     | exception_handler     => fun_exception_handler
+    | exception_delegatee   => fun_exception_delegatee
     | trap_handler          => fun_trap_handler
     | prepare_trap_vector   => fun_prepare_trap_vector
     | tvec_addr             => fun_tvec_addr
+    | handle_illegal        => fun_handle_illegal
     | execute_RTYPE         => fun_execute_RTYPE
     | execute_ITYPE         => fun_execute_ITYPE
     | execute_UTYPE         => fun_execute_UTYPE
@@ -806,6 +904,8 @@ Module RiscvPmpProgramKit <: (ProgramKit RiscvPmpTermKit).
     | execute_RISCV_JALR    => fun_execute_RISCV_JALR
     | execute_LOAD          => fun_execute_LOAD
     | execute_STORE         => fun_execute_STORE
+    | execute_ECALL         => fun_execute_ECALL
+    | execute_MRET          => fun_execute_MRET
     end.
 
 End RiscvPmpProgramKit.
